\documentclass[12pt]{article}
\usepackage[russian]{babel}
\usepackage{amsmath}

\begin{document}

\begin{multline}
1+2+3+4+\ldots\\
+46+47+48+\ldots\\
+99+100=5050
\end{multline}

\begin{gather}
2\times 2=4\\
9\times 9=81
\end{gather}

\begin{equation}
\begin{split}
1999&=1000+900+{}\\
&+90+9
\end{split}
\end{equation}

\begin{align}
7\times 9& =63 & 63:9& =7\\
9\times 10& =90 & 90:10& =9
\end{align}

\begin{align*}
3\cdot 5+7\cdot 5&=(3+7)
\cdot5 &&\text{(ясно)}\\
&=50&&\text{(очевидно)}
\end{align*}

\begin{align**}
3\cdot 5+7\cdot 5&=(3+7)
\cdot5 &&\text{(ясно)}\\
&=50&&\text{(очевидно),}\\
\intertext{откуда}
15+35 &=50
\end{align**}

$$
\left\{
\begin{aligned}
x^2+y^2&=7\\
x+y & = 3.\\
\end{aligned}
\right.
$$

$$
|x|=\begin{cases}
x,&\text{если $x>0$;}\\
0,&\text{если $x=0$;}\\
-x,&\text{если $x<0$.}
\end{cases}
$$

$$
\left\{
\begin{array}{rcl}
x^2+y^2&=&7\\
x+y & = &3.\\
\end{array}
\right.
$$

\begin{eqnarray}
2\times3&=&6\\
2+3&=&5\label{silly}
\end{eqnarray}
На с. ~\pageref{silly}
приведено глупое уравнение ~\ref{silly}.

\begin{eqnarray}
\int_{-\infty}^\infty
e^{-x^2}dx & = &
\sqrt{\pi}\nonumber\\
\sqrt{576} & = & 24
\end{eqnarray}

$$
a^{1-\sigma}b^\sigma \leq (1-\sigma)a+\sigma b. \eqno(1.1)
$$

$$
\left| \sum_{i=1}^n x_iy_i \right| \leq \sum_{i=1}^n |x_i||y_i| \leq \left( \sum_{i=1}^n |x_i|^{\frac1{1-\sigma}} \right)^{1-\sigma} \left( \sum_{i=1}^n |y_i|^{\frac1\sigma} \right)^\sigma . \eqno(1.3)
$$

$$
||x||_\sigma = \begin{cases}
\max\limits_{i} |x_i|, &\text{если $\sigma = 0$;} \\
\left( \sum\limits_{i=1}^n |x_i|^{\frac1\sigma} \right)^\sigma , &\text{если $0 < \sigma \leq 1$.} \\
\end{cases}
$$

$$
c_k = \sum\limits_{\begin{split} k_1 \geq 0, \ldots, k_n \geq 0,\\ 1k_1 + \ldots + nk_n = k\\ \end{split}}(-1)^{k_1+\ldots+k_n}\frac{(k_1+\ldots+k_n)!}{k_1!\ldots k_n!}p_1^{k_1}\ldots p_n^{k_n}.
$$

$$
\text{k$(t)$} = \frac1{2\pi i} \int\limits_{\partial\sigma} e^{t\lambda}\text{r}_n(\lambda)d\lambda, \eqno(6)
$$

$$
\text{k$(t)$} = \sum\limits_{j=1}^n e^{t\text{a}_j} \prod\limits_{1\leq k\leq n,k\neq j}^n (\text{a}_j - \text{a}_k)^{-1}. \eqno(7)
$$

$$
S(\text{a}_j) \cap S(\text{a}_k) = 0 \quad \text{при} \quad j \neq k. \eqno(10)
$$

$$
\beta(a, b, c) = \begin{cases}
\frac{-b + \sqrt{b^2 - 4ac}}{2a}, &\text{если $b^2 - 4ac > 0$,}\\
-\frac{b}{2a}, &\text{если $b^2 - 4ac \leq 0$.}\\
\end{cases} \leqno(13)
$$

$$
\text{Re}a_{ii} + \left( \sum\limits_{j\neq i} h_i^{-1}|a_{ij}|h_j \right)^{1-\alpha} \left( \sum\limits_{j\neq i} h_j^{-1}|a_{ji}|h_i \right)^{\alpha} <0, i = 1, 2, \ldots, n. \eqno(10.7)
$$

$$
\frac1{2\pi i} \int\limits_{\partial\sigma} f(\lambda) \text{r}_n(\lambda)d\lambda = \sum\limits_{j=1}^n f(\text{a}_j) \text{c}_{jn}. \eqno(20)
$$

\end{document} 